

$$1) \quad a) \quad T = \frac{1}{2} m l^2 \dot{\theta}^2 \quad U = mgl(1 - \cos \theta)$$

$$P_{\theta} = \frac{\partial T}{\partial \dot{\theta}} = m l^2 \dot{\theta}$$

b)

$$\dot{\theta} = \frac{P_{\theta}}{m l^2}, \quad T = \frac{1}{2} m l^2 \frac{P_{\theta}^2}{m^2 l^4} = \frac{P_{\theta}^2}{2 m l^2}$$

$$c) \quad H = \frac{P_{\theta}^2}{2m} + mgl(1 - \cos \theta)$$

$$\dot{\theta} = \frac{\partial H}{\partial P_{\theta}} = \frac{P_{\theta}}{m l^2} \quad \dot{P}_{\theta} = \frac{-\partial H}{\partial \theta} = -mgl \sin \theta$$

d)

$$\ddot{\theta} = \frac{\dot{P}_{\theta}}{m l^2} = \frac{-mgl \sin \theta}{m l^2} = -\frac{g}{l} \sin \theta$$

$$\sin \theta \approx \theta$$

$$\ddot{\theta} = -\frac{g}{l} \theta = -\omega^2 \theta, \quad \omega = \sqrt{\frac{g}{l}}$$

2

$$a) T = \frac{1}{2} m (\dot{x}^2 + \dot{y}^2), \quad U = \frac{1}{2} k (x^2 + y^2) + \lambda xy.$$

b)

$$\begin{aligned} p_x &= \frac{\partial T}{\partial \dot{x}} = m \dot{x} & \dot{x} &= \frac{p_x}{m} & T &= \frac{1}{2} m \left(\frac{p_x^2}{m^2} + \frac{p_y^2}{m^2} \right) \\ p_y &= \frac{\partial T}{\partial \dot{y}} = m \dot{y} & \dot{y} &= \frac{p_y}{m} & &= \frac{p_x^2 + p_y^2}{2m} \end{aligned}$$

$$c) H = \frac{p_x^2 + p_y^2}{2m} + \frac{1}{2} k (x^2 + y^2) + \lambda xy$$

d)

$$\dot{x} = \frac{\partial H}{\partial p_x} = \frac{p_x}{m} \quad \dot{y} = \frac{\partial H}{\partial p_y} = \frac{p_y}{m}$$

$$\dot{p}_x = -\frac{\partial H}{\partial x} = -kx - \lambda y \quad \dot{p}_y = -\frac{\partial H}{\partial y} = -ky - \lambda x$$

$$\ddot{x} = \frac{\dot{p}_x}{m} = -\frac{k}{m} x - \frac{\lambda}{m} y \quad \ddot{y} = \frac{\dot{p}_y}{m} = -\frac{k}{m} y - \frac{\lambda}{m} x$$